Veir/PatternRewriter/Semantics.lean
@@ -1,0 +1,261 @@
+import Veir.PatternRewriter.Basic
+import Veir.Interpreter.WellFormed
+import Veir.IR.WellFormed
+import Veir.Rewriter.WellFormed.Builder
+import Veir.Rewriter.GetSetInBounds
+
+namespace Veir
+
+def LocalRewritePattern.ReturnOpsWf
+  (pattern : LocalRewritePattern OpCode) : Prop :=
+  ∀ ctx (op : OperationPtr),
+  ∀ newCtx newOps newValues, pattern ctx op = some (newCtx, some (newOps, newValues)) →
+  ∀ newOp ∈ newOps, newOp.InBounds newCtx ∧ ¬newOp.InBounds ctx
+
+def LocalRewritePattern.WellFormedContext
+  (pattern : LocalRewritePattern OpCode) : Prop :=
+  ∀ ctx (op : OperationPtr),
+  ctx.WellFormed →
+  ∀ newCtx newOps newValues, pattern ctx op = some (newCtx, some (newOps, newValues)) →
+  newCtx.WellFormed
+
+def LocalRewritePattern.MatchValues (pattern : LocalRewritePattern OpCode) : Prop :=
+  ∀ ctx (op : OperationPtr) (_ : op.InBounds ctx),
+  ∀ newCtx newOps newValues, pattern ctx op = some (newCtx, some (newOps, newValues)) →
+  newValues.size = op.getNumResults! ctx
+
+def LocalRewritePattern.PreservesSemantics
+  (pattern : LocalRewritePattern OpCode)
+  (safePattern : pattern.ReturnOpsWf)
+  (patternWfCtx : pattern.WellFormedContext)
+  (_ : pattern.MatchValues) : Prop :=
+  ∀ ctx (ctxWf : ctx.WellFormed) (op : OperationPtr) (opInBounds : op.InBounds ctx),
+  ∀ newCtx newOps newValues (hpattern : pattern ctx op = some (newCtx, some (newOps, newValues))),
+  ∀ (state : InterpreterState), state.WellFormed ctx →
+  ∀ newState cf, interpretOp ctx op state = some (newState, cf) →
+  ∃ newState',
+    interpretOpList' newCtx newOps.toList state (by grind [ReturnOpsWf]) (by grind [WellFormedContext]) = some (newState', cf) ∧
+    ∀ idx (hIdx : idx < newValues.size),
+      newState.getVar? (op.getResult idx) = newState'.getVar? newValues[idx]
+
+
+namespace Example
+
+def matchOp (op : OperationPtr) (ctx : IRContext OpCode) (opType : OpCode) (numOperands : Nat) :
+    Option (Array ValuePtr × propertiesOf opType) := do
+  guard (op.getOpType! ctx = opType)
+  guard (op.getNumOperands! ctx = numOperands)
+  guard (op.getNumResults! ctx = 1)
+  let operands := op.getOperands! ctx
+  some (operands, op.getProperties! ctx opType)
+
+theorem matchOp_implies (opInBounds : op.InBounds ctx) :
+  matchOp op ctx opType numOperands = some (operands, properties) →
+  op.getOpType! ctx = opType ∧
+  op.getNumOperands! ctx = numOperands ∧
+  op.getNumResults! ctx = 1 ∧
+  operands = op.getOperands! ctx ∧
+  properties = op.getProperties! ctx opType := by
+  simp only [matchOp]
+  simp only [guard, Option.pure_def, Option.bind_eq_bind, Option.bind_eq_some_iff, ite_eq_left_iff,
+    reduceCtorEq, imp_false, Decidable.not_not, Option.some.injEq, Prod.mk.injEq, exists_const,
+    and_imp]
+  intros
+  grind
+
+theorem matchOp_interpretOp
+  (opInBounds : op.InBounds ctx) :
+  matchOp op ctx opType numOperands = some (operands, properties) →
+  interpretOp ctx op state = some (newState, cf) →
+  ∃ values newValue,
+    operands.mapM state.getVar? = some values ∧
+    interpretOp' opType properties ((op.get! ctx).results.map (·.type)) values = some (#[newValue], cf) ∧
+    newState = state.setVar (op.getResult 0) newValue := by
+  intro hmatch hinterp
+  have ⟨hOpType, hNumOperands, hNumResults, hOperands, hProperties⟩ := matchOp_implies opInBounds hmatch
+  simp only [interpretOp] at hinterp
+  simp only [Option.pure_def, Option.bind_eq_bind, Option.bind_eq_some_iff, Option.some.injEq,
+    Prod.mk.injEq, Prod.exists, exists_eq_right_right] at hinterp
+  have ⟨values, hValues, resValues, hInterpOp', hNewState⟩ := hinterp; clear hinterp
+  exists values
+  subst operands
+  simp [InterpreterState.getOperandValues] at hValues
+  simp only [hValues, true_and]
+  have : resValues.size = 1 := by sorry -- Missing lemma about number of results and interpretation
+  exists resValues[0]
+  have : resValues = #[resValues[0]] := by grind
+  grind [InterpreterState.setResultValues, InterpreterState.setResultValues_loop]
+
+
+def matchAddi (op : OperationPtr) (ctx : IRContext OpCode) : Option (ValuePtr × ValuePtr × propertiesOf .arith_addi) := do
+  let (op, properties) ← matchOp op ctx .arith_addi 2
+  return (op[0]!, op[1]!, properties)
+
+theorem matchAddi_implies (opInBounds : op.InBounds ctx) :
+  matchAddi op ctx = some (lhs, rhs, properties) →
+  op.getOpType! ctx = .arith_addi ∧
+  op.getNumResults! ctx = 1 ∧
+  op.getOperands! ctx = #[lhs, rhs] ∧
+  properties = op.getProperties! ctx .arith_addi := by
+  intro hmatch
+  simp only [matchAddi, Option.pure_def, Option.bind_eq_bind, Option.bind_eq_some_iff,
+    Option.some.injEq, Prod.mk.injEq, Prod.exists] at hmatch
+  grind [matchOp_implies]
+
+theorem matchAddi_interpretOp
+  (opInBounds : op.InBounds ctx) :
+  matchAddi op ctx = some (lhs, rhs, properties) →
+  interpretOp ctx op state = some (newState, cf) →
+  ∃ lhsVal rhsVal newValue,
+    state.getVar? lhs = some lhsVal ∧
+    state.getVar? rhs = some rhsVal ∧
+    interpretOp' .arith_addi properties #[((op.getResult 0).get! ctx).type] #[lhsVal, rhsVal] = some (#[newValue], cf) ∧
+    newState = state.setVar (op.getResult 0) newValue := by
+  intro hmatch
+  simp only [matchAddi, Option.pure_def, Option.bind_eq_bind, Option.bind_eq_some_iff,
+    Option.some.injEq, Prod.mk.injEq, Prod.exists] at hmatch
+  have ⟨operands, properties, hmatchOp, hlhs, hrhs, hprop⟩ := hmatch
+  have ⟨hOpType, hNumOperands, hNumResults, hOperands, hProperties⟩ := matchOp_implies opInBounds hmatchOp
+  intro hinterp
+  have ⟨values, newValue, hValues, hinterp', hnewState⟩ := matchOp_interpretOp opInBounds hmatchOp hinterp
+  have : operands = #[lhs, rhs] := by grind
+  subst this
+  simp only [List.mapM_toArray, List.mapM_cons, List.mapM_nil, Option.pure_def, Option.bind_eq_bind,
+    Option.bind_some, Option.map_eq_map, Option.map_bind, Option.bind_eq_some_iff,
+    Function.comp_apply, Option.some.injEq, Option.map_some] at hValues
+  have : #[((op.getResult 0).get! ctx).type] = (op.get! ctx).results.map (·.type) := by sorry
+  grind
+
+def matchConstantOp (op : OperationPtr) (ctx : IRContext OpCode) : Option IntegerAttr := do
+  let .arith_constant := op.getOpType! ctx | none
+  let properties := op.getProperties! ctx .arith_constant
+  return properties.value
+
+def matchConstantVal (val : ValuePtr) (ctx : IRContext OpCode) : Option IntegerAttr := do
+  let .opResult opResultPtr := val | none
+  let op := opResultPtr.op
+  matchConstantOp op ctx
+
+theorem matchConstantVal_opRes :
+    matchConstantVal val ctx = some cst →
+    ∃ op,
+      val = .opResult (op.getResult 0) ∧
+      matchConstantOp op ctx = some cst := by
+  sorry -- Missing lemmas about constant and number of results
+
+theorem matchConstantVal_state_get {state : InterpreterState} :
+    matchConstantVal val ctx = some cst →
+    state.WellFormed ctx →
+    state.getVar? val = some value →
+    value = .int cst.type.bitwidth (.val (BitVec.ofNat cst.type.bitwidth cst.value.toNat)) := by
+  intro hMatch stateWf stateVar
+  have ⟨op, hVal, hConst⟩ := matchConstantVal_opRes hMatch
+  subst val
+  simp only [InterpreterState.WellFormed] at stateWf
+  have eqLemma := stateWf (op.getResult 0) (by sorry) value stateVar
+  simp only [InterpreterState.SatisfiesEquationLemma] at eqLemma
+  have ⟨cf, hinterp⟩ := eqLemma
+  simp [interpretOp] at hinterp
+  sorry -- Just have to continue more here
+
+def addIConstantFolding (ctx: IRContext OpCode) (op: OperationPtr) :
+    Option (IRContext OpCode × Option (Array OperationPtr × Array ValuePtr)) := do
+  -- Match an `arith.addi`
+  let (lhs, rhs, _) ← matchAddi op ctx
+  let lhsConst ← matchConstantVal lhs ctx
+  let rhsConst ← matchConstantVal rhs ctx
+
+  -- Sum both constant values
+  let newConst := ArithConstantProperties.mk (IntegerAttr.mk ((lhsConst.value + rhsConst.value) % 2 ^ 32) (IntegerType.mk 32))
+  let (ctx, newOp) ← Rewriter.createOp ctx .arith_constant #[IntegerType.mk 32] #[] #[] #[] newConst none sorry sorry sorry sorry sorry
+  return (ctx, some (#[newOp], #[newOp.getResult 0]))
+
+
+theorem addIConstantFolding_returnOpsWf :
+    LocalRewritePattern.ReturnOpsWf addIConstantFolding := by
+  simp only [LocalRewritePattern.ReturnOpsWf, addIConstantFolding]
+  intro ctx op newCtx newOps newValues
+  simp [Option.bind_eq_some_iff]
+  intro lhs rhs _ hMatchAdd lhsConst matchLhs rhsConst matchRhs newCtx' newOp hNewCtx _ _ _ newOp'
+  subst newCtx' newOps newValues
+  simp only [List.mem_toArray, List.mem_cons, List.not_mem_nil, or_false]
+  intro _; subst newOp'
+  constructor -- Missing InBounds lemmas
+  · sorry
+  · sorry
+
+theorem addIConstantFolding_wellFormedContext :
+    LocalRewritePattern.WellFormedContext addIConstantFolding := by
+  simp only [LocalRewritePattern.WellFormedContext, addIConstantFolding]
+  intro ctx op ctxWf newCtx newOps
+  simp only [Option.pure_def, Option.bind_eq_bind, Option.bind_eq_some_iff, Option.some.injEq,
+    Prod.mk.injEq, Prod.exists, forall_exists_index, and_imp]
+  intro newValues lhs rhs _ hMatchAdd lhsConst matchLhs rhsConst matchRhs newCtx' newOp hNewCtx _ _ _
+  subst newCtx' newOps newValues
+  apply Rewriter.createOp_WellFormed _ hNewCtx
+  grind
+
+theorem addIConstantFolding_matchValues :
+    LocalRewritePattern.MatchValues addIConstantFolding := by
+  simp only [LocalRewritePattern.MatchValues, addIConstantFolding]
+  intro ctx op opInBounds newCtx newOps
+  simp [Option.bind_eq_some_iff]
+  intro newValues lhs rhs _ hMatchAdd lhsConst matchLhs rhsConst matchRhs newCtx' newOp hNewCtx _ _ _
+  subst newCtx' newOps newValues
+  have := matchAddi_implies (by sorry) hMatchAdd
+  grind
+
+theorem addIConstantFolding_preservesSemantics :
+    LocalRewritePattern.PreservesSemantics addIConstantFolding addIConstantFolding_returnOpsWf addIConstantFolding_wellFormedContext addIConstantFolding_matchValues := by
+  -- Unfold definition and cleanup hypotheses
+  simp only [LocalRewritePattern.PreservesSemantics, addIConstantFolding]
+  intro ctx ctxWf op opInBounds newCtx newOps newValues hpattern state stateWf newState cf hinterp
+  simp only [Option.pure_def, Option.bind_eq_bind, Option.bind_eq_some_iff, Option.some.injEq,
+    Prod.mk.injEq, Prod.exists] at hpattern
+  have ⟨lhs, rhs, properties, matchAdd, lhsConst, matchLhs, rhsConst, matchRhs, newCtx', newOp, hNewCtx, _, _, _⟩ := hpattern; clear hpattern
+  subst newCtx' newOps newValues
+
+  -- Unfold interpretation of the original add operation parametrized by the lhs and rhs values
+  have ⟨hAddOpCode, hOpNumResults, hOpOperands, hOpProperties⟩ := matchAddi_implies opInBounds matchAdd
+  have ⟨lhsVal, rhsVal, newValue, hLhsVal, hRhsVal, hInterpOp, hNewState⟩ := matchAddi_interpretOp opInBounds matchAdd hinterp
+  subst hNewState
+  have lhsValDef := matchConstantVal_state_get matchLhs stateWf hLhsVal
+  have rhsValDef := matchConstantVal_state_get matchRhs stateWf hRhsVal
+  subst lhsVal rhsVal
+  simp only [interpretOp', ne_eq, Option.pure_def, dite_not, Option.dite_none_right_eq_some,
+    Option.some.injEq, Prod.mk.injEq, Array.mk.injEq, List.cons.injEq, and_true,
+    exists_and_right] at hInterpOp
+  have ⟨⟨eqBitwidths, hNewValue⟩, hcf⟩ := hInterpOp; subst cf
+
+  -- Unfold interpretation of new operation
+  simp only [List.size_toArray, List.length_cons, List.length_nil, Nat.zero_add, Nat.lt_one_iff,
+    List.getElem_toArray, List.getElem_singleton, forall_eq]
+  simp only [InterpreterState.getVar?_setVar, ↓reduceIte]
+  simp only [interpretOpList', interpretOp]
+  have newOpOperands : state.getOperandValues newCtx newOp = some #[] := by sorry -- Missing lemma
+  have newOpType : newOp.getOpType! newCtx = .arith_constant := by sorry -- Missing lemma
+  simp only [newOpOperands, Option.pure_def, Option.bind_eq_bind, Option.bind_some]
+  simp [interpretOp']; rw [newOpType]
+  simp only
+  have ⟨res0, hres0⟩ : ∃ opr, (newOp.get! newCtx).results[0]? = some opr := by sorry -- Missing lemmas
+  have : res0.type.val = .integerType (IntegerType.mk 32) := by sorry -- Missing lemma about createOp and result types
+  simp only [hres0, Option.map_some, Option.bind_some, this, Option.some.injEq, Prod.mk.injEq,
+    and_true, exists_eq_left']
+  have : newOp.getNumResults! newCtx = 1 := by sorry -- Missing lemma
+  simp only [InterpreterState.setResultValues, this, InterpreterState.setResultValues_loop,
+    List.size_toArray, List.length_cons, List.length_nil, Nat.zero_add, Nat.lt_add_one,
+    getElem!_pos, List.getElem_toArray, List.getElem_cons_zero]
+
+  -- actual proof of the rewrite
+  subst newValue
+  simp only [InterpreterState.getVar?_setVar, ↓reduceIte, Option.some.injEq,
+    RuntimeValue.int.injEq]
+  have lhsBitwidth : lhsConst.type.bitwidth = 32 := by sorry -- TODO
+  simp only [lhsBitwidth, true_and]
+  have : (newOp.getProperties! newCtx .arith_constant) = { value := { value := (lhsConst.value + rhsConst.value) % 2 ^ 32, type := { bitwidth := 32 } } } := by sorry
+  simp only [this]
+  rw [HAdd.hAdd, instHAdd]
+  simp only [Add.add, Data.LLVM.Int.add, Data.LLVM.Int.cast, BitVec.cast_ofNat]
+  rw [lhsBitwidth]
+  congr
+  sorry
